some fresh stuff

src/burrow/fresh.v
@@ -11,7 +11,96 @@ Section Fresh.
 
 Context {M} `{!EqDecision M} `{!TPCM M}.
 
-Definition is_fresh_nat : Branch M -> nat -> Prop. Admitted.
+Fixpoint node_no_idx (node: Node M) (f: nat) (idx: nat) : Prop :=
+  match node with
+  | CellNode _ branch =>
+         f ≠ idx
+      /\ branch_no_idx branch f 0
+  end
+with branch_no_idx (branch: Branch M) (f: nat) (idx: nat) : Prop :=
+  match branch with
+  | BranchNil => True
+  | BranchCons node branch =>
+         node_no_idx node f idx
+      /\ branch_no_idx branch f (S idx)
+  end
+.
+
+Fixpoint node_max_idx (node: Node M) (idx: nat) : nat :=
+  match node with
+  | CellNode _ branch =>
+         idx `max` branch_max_idx branch 0
+  end
+with branch_max_idx (branch: Branch M) (idx: nat) : nat :=
+  match branch with
+  | BranchNil => 1
+  | BranchCons node branch =>
+         node_max_idx node idx `max` branch_max_idx branch (S idx)
+  end
+.
+
+Lemma node_no_idx_rewrite (node: Node M) (f: nat) (idx: nat)
+    : node_no_idx node f idx =
+  match node with
+  | CellNode _ branch =>
+         f ≠ idx
+      /\ branch_no_idx branch f 0
+  end. Proof. unfold node_no_idx, branch_no_idx. destruct node. trivial. Qed.
+  
+Lemma branch_no_idx_rewrite (branch: Branch M) (f: nat) (idx: nat)
+    : branch_no_idx branch f idx =
+  match branch with
+  | BranchNil => True
+  | BranchCons node branch =>
+         node_no_idx node f idx
+      /\ branch_no_idx branch f (S idx)
+  end
+.
+Proof. unfold branch_no_idx, node_no_idx. destruct branch; trivial. Qed.
+
+Lemma node_max_idx_rewrite (node: Node M) (idx: nat)
+  : node_max_idx node idx =
+  match node with
+  | CellNode _ branch =>
+         idx `max` branch_max_idx branch 0
+  end.
+Proof. unfold branch_max_idx, node_max_idx. destruct node; trivial. Qed.
+  
+Lemma branch_max_idx_rewrite (branch: Branch M) (idx: nat)
+  : branch_max_idx branch idx =
+  match branch with
+  | BranchNil => 1
+  | BranchCons node branch =>
+         node_max_idx node idx `max` branch_max_idx branch (S idx)
+  end
+.
+Proof. unfold branch_no_idx, node_no_idx. destruct branch; trivial. Qed.
+
+Lemma node_no_idx_of_gt_max (node: Node M) (idx: nat) (t: nat)
+    (gt: t > node_max_idx node idx) : node_no_idx node t idx
+with branch_no_idx_of_gt_max (branch: Branch M) (idx: nat) (t: nat)
+    (gt: t > branch_max_idx branch idx) : branch_no_idx branch t idx.
+Proof.
+  - destruct node.
+    have ihb := branch_no_idx_of_gt_max b.
+    clear node_no_idx_of_gt_max.
+    clear branch_no_idx_of_gt_max.
+    rewrite node_no_idx_rewrite. rewrite node_max_idx_rewrite in gt. split.
+    + lia.
+    + apply ihb. lia.
+  - destruct branch.
+    + have ihb := branch_no_idx_of_gt_max branch.
+      have ihn := node_no_idx_of_gt_max n.
+      clear node_no_idx_of_gt_max.
+      clear branch_no_idx_of_gt_max.
+      rewrite branch_no_idx_rewrite. rewrite branch_max_idx_rewrite in gt.
+      split.
+      * apply ihn. lia.
+      * apply ihb. lia.
+    + unfold branch_no_idx. trivial.
+Qed.
+  
+Definition is_fresh_nat (b: Branch M) (f: nat) : Prop := branch_no_idx b f 0.
 
 Definition alloc_alpha
     {RI} `{!EqDecision RI, !Countable RI, !RefinementIndex M RI}
@@ -31,8 +120,36 @@ Lemma trivial_node_at_fresh (b: Branch M) p i
   (is_fresh: is_fresh_nat b i)
   : node_trivial (node_of_pl b (p, i)). Admitted.
   
+Lemma node_no_idx_of_op (node1 node2 : Node M) (f: nat) (idx: nat)
+  (nni: node_no_idx (node1 ⋅ node2) f idx) : node_no_idx node2 f idx
+with branch_no_idx_of_op (branch1 branch2 : Branch M) (f: nat) (idx: nat)
+  (bni: branch_no_idx (branch1 ⋅ branch2) f idx) : branch_no_idx branch2 f idx.
+Proof.
+  - destruct node2.
+    have ihb := branch_no_idx_of_op _ b.
+    clear node_no_idx_of_op.
+    clear branch_no_idx_of_op.
+    rewrite node_no_idx_rewrite. rewrite node_no_idx_rewrite in nni. destruct node1.
+      unfold "⋅", node_op in nni. destruct_ands. split; trivial.
+      apply ihb with (b0 := b0). trivial.
+  - destruct branch2.
+    + have ihb := branch_no_idx_of_op _ branch2.
+      have ihn := node_no_idx_of_op _ n.
+      clear node_no_idx_of_op.
+      clear branch_no_idx_of_op.
+      rewrite branch_no_idx_rewrite. rewrite branch_no_idx_rewrite in bni. destruct branch1.
+      * unfold "⋅", branch_op in bni. destruct_ands. split; trivial.
+        -- apply ihn with (n0 := n0). trivial.
+        -- apply ihb with (b := branch1). trivial.
+      * unfold "⋅", branch_op in bni. trivial.
+    + unfold branch_no_idx. trivial.
+Qed.
+  
 Lemma is_fresh_nat_of_op (a b : Branch M) (i: nat)
-  : is_fresh_nat (a ⋅ b) i -> is_fresh_nat b i. Admitted.
-
+  : is_fresh_nat (a ⋅ b) i -> is_fresh_nat b i. 
+Proof.
+  unfold is_fresh_nat.
+  apply branch_no_idx_of_op.
+Qed.
 
 End Fresh.
